Examples.v
@@ -1,0 +1,81 @@
+From Coq Require Import Strings.String.
+From Coq Require Import Lists.List.
+Open Scope string_scope.
+
+From Elo Require Import Core.
+
+Definition example1 : tm := <{
+  let "m1" : x&w&Nat = new (new (nat 3) : w&Nat) : x&w&Nat in
+  let "m2" : x&w&Nat = new (new (nat 5) : w&Nat) : x&w&Nat in
+  spawn (
+    acq (var "m1") "x" (
+      let "result" : Nat = *(var "x") in (
+        (var "x") := (nat 6);
+        (var "result")
+      )
+    )
+  );
+  spawn (
+    acq (var "m2") "y" (
+      let "result" : Nat = *(var "y") in (
+        (var "y") := (nat 10);
+        (var "result")
+      )
+    )
+  );
+  (nat 20)
+}>.
+
+Ltac solve_ty :=
+  repeat match goal with
+  | |- _ |-- <{unit        }> is _ => eapply T_unit
+  | |- _ |-- <{nat _       }> is _ => eapply T_nat
+  | |- _ |-- <{_; _        }> is _ => eapply T_seq
+  | |- _ |-- <{var _       }> is _ => eapply T_var
+  | |- _ |-- <{fn _ _ _    }> is _ => eapply T_fun
+  | |- _ |-- <{call _ _    }> is _ => eapply T_call
+  | |- _ |-- <{new _ : r&?T}> is _ => eapply T_newR
+  | |- _ |-- <{new _ : x&?T}> is _ => eapply T_newX
+  | |- _ |-- <{new _ : w&?T}> is _ => eapply T_newW
+  (*
+  | T_loadR : forall Gamma t T, Gamma |-- <{*t}> is `Safe T`
+  | T_loadW : forall Gamma t T, Gamma |-- <{*t}> is T
+  *)
+  | |- _ |-- <{_ := _      }> is _ => eapply T_asg
+  | |- _ |-- <{acq _ _ _   }> is _ => eapply T_acq
+  | |- _ |-- <{spawn _     }> is _ => eapply T_spawn
+  end.
+
+Lemma example1_is_well_typed :
+  empty |-- example1 is `Nat`.
+Proof.
+  unfold example1. solve_ty.
+  - unfold safe. simpl. reflexivity.
+  - unfold safe. simpl. reflexivity.
+  - rewrite lookup_update_eq. reflexivity.
+  - eapply T_loadW. solve_ty. rewrite lookup_update_eq. reflexivity.
+  - unfold safe. simpl. reflexivity.
+  - rewrite lookup_update_neq; try solve [intros F; invc F].
+    rewrite lookup_update_eq. reflexivity.
+  - rewrite lookup_update_eq. reflexivity.
+  - eapply T_loadW. solve_ty. rewrite lookup_update_eq. reflexivity.
+Qed.
+
+Lemma example1_reduces_correctly : forall m ths,
+  m = (
+    (Some <{nat 6     }>, `w&Nat`,   false, R_ad  1) ::
+    (Some <{&0 : w&Nat}>, `x&w&Nat`, false, R_tid 0) ::
+    (Some <{nat 10    }>, `w&Nat`,   false, R_ad  3) ::
+    (Some <{&2 : w&Nat}>, `x&w&Nat`, false, R_tid 0) ::
+    nil) -> 
+  ths = (
+    <{nat 6 }> ::
+    <{nat 10}> ::
+    <{nat 20}> ::
+    nil) ->
+  exists tc, base_m / (base_t example1) ~~[tc]~~>* m / ths.
+Proof.
+  unfold base_m, base_t. intros. eexists.
+  eapply multistep_trans.
+Abort.
+
