NoCR.v
@@ -7,6 +7,9 @@ From Elo Require Import Core.
 Inductive no_cr (ad : addr) : tm -> Prop :=
   | nocr_unit  :                 no_cr ad <{unit          }>
   | nocr_nat   : forall n,       no_cr ad <{nat n         }>
+  | nocr_seq   : forall t1 t2,   no_cr ad t1 ->
+                                 no_cr ad t2 ->
+                                 no_cr ad <{t1; t2        }>
   | nocr_var   : forall x,       no_cr ad <{var x         }>
   | nocr_fun   : forall x Tx t,  no_cr ad t  ->
                                  no_cr ad <{fn x Tx t     }>
@@ -39,6 +42,7 @@ Local Ltac _nocr tt :=
   match goal with
   | H : no_cr _   <{unit        }> |- _ => clear H
   | H : no_cr _   <{nat _       }> |- _ => clear H
+  | H : no_cr _   <{_; _        }> |- _ => tt H
   | H : no_cr _   <{var _       }> |- _ => clear H
   | H : no_cr _   <{fn _ _ _    }> |- _ => tt H
   | H : no_cr _   <{call _ _    }> |- _ => tt H
@@ -153,7 +157,11 @@ Definition no_crs (t : tm) := forall ad, no_cr ad t.
 Local Ltac solve_inv_nocrs :=
   unfold no_crs; intros * H; try split; intros; spec; invc_nocr; auto.
 
-Local Lemma inv_nocrs_fun : forall x Tx t,
+Local Lemma inv_nocrs_fun : forall t1 t2,
+  no_crs <{t1; t2}> -> no_crs t1 /\ no_crs t2.
+Proof. solve_inv_nocrs. Qed.
+
+Local Lemma inv_nocrs_seq : forall x Tx t,
   no_crs <{fn x Tx t}> -> no_crs t.
 Proof. solve_inv_nocrs. Qed.
 
@@ -193,17 +201,18 @@ Ltac invc_nocrs :=
   match goal with
   | H : no_crs <{unit        }> |- _ => clear H
   | H : no_crs <{nat _       }> |- _ => clear H
+  | H : no_crs <{_; _        }> |- _ => eapply inv_nocrs_seq   in H as [? ?]
   | H : no_crs <{var _       }> |- _ => clear H
-  | H : no_crs <{fn _ _ _    }> |- _ => eapply inv_nocrs_fun    in H
-  | H : no_crs <{call _ _    }> |- _ => eapply inv_nocrs_call   in H as [? ?]
+  | H : no_crs <{fn _ _ _    }> |- _ => eapply inv_nocrs_fun   in H
+  | H : no_crs <{call _ _    }> |- _ => eapply inv_nocrs_call  in H as [? ?]
   | H : no_crs <{& _ : _     }> |- _ => clear H
-  | H : no_crs <{new _ : _   }> |- _ => eapply inv_nocrs_new    in H
-  | H : no_crs <{init _ _ : _}> |- _ => eapply inv_nocrs_init   in H
-  | H : no_crs <{* _         }> |- _ => eapply inv_nocrs_load   in H
-  | H : no_crs <{_ := _      }> |- _ => eapply inv_nocrs_asg    in H as [? ?]
-  | H : no_crs <{acq _ _ _   }> |- _ => eapply inv_nocrs_acq    in H as [? ?]
-  | H : no_crs <{cr _ _      }> |- _ => eapply inv_nocrs_cr     in H; auto
-  | H : no_crs <{spawn _     }> |- _ => eapply inv_nocrs_spawn  in H
+  | H : no_crs <{new _ : _   }> |- _ => eapply inv_nocrs_new   in H
+  | H : no_crs <{init _ _ : _}> |- _ => eapply inv_nocrs_init  in H
+  | H : no_crs <{* _         }> |- _ => eapply inv_nocrs_load  in H
+  | H : no_crs <{_ := _      }> |- _ => eapply inv_nocrs_asg   in H as [? ?]
+  | H : no_crs <{acq _ _ _   }> |- _ => eapply inv_nocrs_acq   in H as [? ?]
+  | H : no_crs <{cr _ _      }> |- _ => eapply inv_nocrs_cr    in H; auto
+  | H : no_crs <{spawn _     }> |- _ => eapply inv_nocrs_spawn in H
   end.
 
 (* lemmas ------------------------------------------------------------------ *)
